src/coq/Transformations/Transform.v
@@ -8,7 +8,7 @@ Open Scope string_scope.
 Definition mangle_raw_id (id:raw_id) : raw_id :=
   match id with
   | Anon n => id
-  | Name s => Name (append "_vellvm" s)
+  | Name s => Name (append "_twophase" s)
   | Raw n => id
   end.
 
