src/coq/Utils/NoEvent.v
@@ -1086,5 +1086,5 @@ Module PICK_REMOVE (ADDR : ADDRESS) (IP : INTPTR) (SIZE : Sizeof) (Events : LLVM
   Import Events.
 
   Variable remove_pick_ub : itree (ExternalCallE +' PickUvalueE +' UBE +' DebugE +' FailureE) ~> itree (ExternalCallE +' DebugE +' FailureE).
-  Variable deterministic_vellvm : forall R, itree L0 R -> Prop.
+  Variable deterministic_twophase : forall R, itree L0 R -> Prop.
 End PICK_REMOVE.
